utils/Zeta.BinTreePtr.fsti
@@ -166,8 +166,8 @@ val lemma_extend_not_reachable
                    not (points_to_some pf a (desc_dir d a)) /\
                    root_reachable pf a})
   (n: bin_tree_node):
-  Lemma (requires (not (root_reachable pf n) /\ n <> d))
-        (ensures (not (root_reachable (extend_ptrfn pf d a) n)))
+  Lemma (requires (n <> d))
+        (ensures (not (root_reachable pf n) ==> not (root_reachable (extend_ptrfn pf d a) n)))
 
 (* Extend the pointer function by cutting a pointer *)
 let extendcut_ptrfn 
